theories/heap_lang/notation.v
@@ -58,22 +58,28 @@ Notation "'if:' e1 'then' e2 'else' e3" := (If e1%E e2%E e3%E)
   (at level 200, e1, e2, e3 at level 200) : expr_scope.
 Notation "'iffun:' e0 'as' x => e1 'else' e2" :=
   (Match (UnOp FunofOp e0) BAnon e2 x%bind e1)
-  (at level 200, e0, x, e1, e2 at level 200, only parsing) : expr_scope.
+  (at level 200, e0, x, e1, e2 at level 200) : expr_scope.
 Notation "'iflit:' e0 'as' x => e1 'else' e2" :=
   (Match (UnOp LitofOp e0) BAnon e2 x%bind e1)
-  (at level 200, e0, x, e1, e2 at level 200, only parsing) : expr_scope.
+  (at level 200, e0, x, e1, e2 at level 200) : expr_scope.
+Notation "'ifint:' e0 'as' x => e1 'else' e2" :=
+  (Match (UnOp IntofOp e0) BAnon e2 x%bind e1)
+  (at level 200, e0, x, e1, e2 at level 200) : expr_scope.
+Notation "'ifbool:' e0 'as' x => e1 'else' e2" :=
+  (Match (UnOp BoolofOp e0) BAnon e2 x%bind e1)
+  (at level 200, e0, x, e1, e2 at level 200) : expr_scope.
 Notation "'ifloc:' e0 'as' x => e1 'else' e2" :=
   (Match (UnOp LocofOp e0) BAnon e2 x%bind e1)
-  (at level 200, e0, x, e1, e2 at level 200, only parsing) : expr_scope.
+  (at level 200, e0, x, e1, e2 at level 200) : expr_scope.
 Notation "'ifpair:' e0 'as' x  => e1 'else' e2" :=
   (Match (UnOp PairofOp e0) BAnon e2 x%bind e1)
-  (at level 200, e0, x, e1, e2 at level 200, only parsing) : expr_scope.
+  (at level 200, e0, x, e1, e2 at level 200) : expr_scope.
 Notation "'ifinl:' e0 'as' x  => e1 'else' e2" :=
   (Match (UnOp InlofOp e0) BAnon e2 x%bind e1)
-  (at level 200, e0, x, e1, e2 at level 200, only parsing) : expr_scope.
+  (at level 200, e0, x, e1, e2 at level 200) : expr_scope.
 Notation "'ifinr:' e0 'as' x  => e1 'else' e2" :=
   (Match (UnOp InrofOp e0) BAnon e2 x%bind e1)
-  (at level 200, e0, x, e1, e2 at level 200, only parsing) : expr_scope.
+  (at level 200, e0, x, e1, e2 at level 200) : expr_scope.
 
 (** Derived notions, in order of declaration. The notations for let and seq
 are stated explicitly instead of relying on the Notations Let and Seq as
